src/impl/TLS13.Impl.Handle.ChangeCipherSpec.fsti
@@ -31,7 +31,7 @@ fn handle_change_cipher_spec
            B.length 'old_network_out == SZ.v network_out_len /\
            B.length 'old_app_out == SZ.v app_out_len /\
            L.tls_message_is_change_cipher_spec l /\
-           CT.received_tls_raw_delta_legal
+           CT.received_tls_raw_delta_legal_unbuffered
                    'st0
                    M.TlsChangeCipherSpec
                    (Ghost.reveal 'raw_bytes))
